# 2.6: Implicit Differentiation
- Functions that we have covered so far express one variable explicitly in terms of another
- Examples
  - $y = \sqrt{x^3 + 1}$
  - $y = x\sin x$
  - $y = f(x)$ (generally)
- Some functions are defined by an implicit relationship between $x$ and $y$
- Examples
  - $x^2 + y^2 = 25$
  - $x^3 + y^3 = 6xy$ (folium of Descartes)

## Implicit Differentiation
- We don't need to solve an equation for $y$ in terms of $x$ to find the derivative of $y$, but can use the method of **implicit differentiation**
  - This means to differentiate both sides of the equation with respect to $x$ and then solve the resulting equation for $\frac{dy}{dx}$
- Example: Find $\frac{dy}{dx}$ for $x^2 + y^2 = 25$. Then find equation of the tangent to the circle at the point $(3, 4)$
  - Differentiate both sides
    - $\frac{d}{dx}(x^2 + y^2) = \frac{d}{dx}(25)$
    - $\frac{d}{dx}(x^2) + \frac{d}{dx}(y^2) = 0$
      - We have to remember that $y$ is a function of $x$ and use the Chain rule
    - $\frac{d}{dx}(y^2) = \frac{d}{dx}(y^2)\frac{dy}{dx} = 2y\frac{dy}{dx}$
    - $2x + 2y\frac{dy}{dx} = 0$
  - Now solve for $\frac{dy}{dx}$
    - $\frac{dy}{dx} = -\frac{x}{y}$
  - Then we can find our equation of the tangent at $(3, 4)$
    - $\frac{dy}{dx} = -\frac{3}{4}$ (this is our slope)
    - Put into point-slope form: $y - y_1 = m(x - x_1)$
    - $y - 4 = -\frac{3}{4}(x - 3)$ or $3x + 4y = 25$
- Example: Solve the same equation in terms of $y$
  - $x^2 + y^2 = 25 \to y = \pm \sqrt{25 - x^2}$
  - Because the point $(3, 4)$ is on the upper semi-circle, we use $f(x) = \sqrt{25 - x^2}$ and use the chain rule
  - $f'(x) = \frac{1}{2}(25 - x^2)^{-\frac{1}{2}}\frac{d}{dx}(25 - x^2)$
  - $= \frac{1}{2}(25 - x^2)^{-\frac{1}{2}}(-2x) = -\frac{x}{\sqrt{25 - x^2}}$
  - Then use the point $(3, 4)$
    - $f'(3) = -\frac{3}{\sqrt{25 - 3^2}} = -\frac{3}{4}$
- Example: Find $y'$ if $\sin(x + y) = y^2\cos x$
  - Differentiate implicitly with respect to $x$ and remembering that $y$ is a function of $x$, we get
    - $\cos(x + y) \cdot (1 + y') = y^2(-\sin x) + (\cos x)(2yy')$
  - Collect the terms that involve $y'$
    - $\cos(x + y) + y^2\sin x = (2y\cos x)y' - \cos(x + y) \cdot y'$
  - Which gives us
    - $y' = \frac{y^2\sin x + \cos(x + y)}{2y\cos x - \cos(x + y)}$

## Second Derivatives of Implicit Functions
- Example: find $y''\text{ if }x^4 + y^4 = 16$
  - Differentiate implicitly with respect to $x$
    - $4x^3 + 4y^3y' = 0$
      - Step by step:
        - $\frac{d}{dx}(x^4 + y^4) = \frac{d}{dx}(16)$
        - $\frac{d}{dx}(x^4) + \frac{d}{dx}(y^4) = 0$ (derivative of constant is 0)
        - $\frac{d}{dx}(x^4) = 4x^3$ (power rule)
        - Chain rule on $y^4 = (y(x))^4 = \frac{d}{dx}(y^4)\cdot\frac{dy}{dx} = 4y^3 \cdot y'$
        - $4x^3 + 4y^3y' = 0$
    - $y' = -\frac{x^3}{y^3}$ (solve for $y'$)
  - Find $y''$ using the Quotient Rule and remembering that $y$ is a function of $x$
    - $y'' = \frac{d}{dx}(-\frac{x^3}{y^3}) = -\frac{y^3(d/dx)(x^3) - x^3(d/dx)(y^3)}{(y^3)^2}$
    - $= -\frac{y^3\cdot 3x^2 - x^3(3y^2y')}{y^6}$
  - Substitute our original derivative in ($-\frac{x^3}{y^3}$)
    - $y'' = -\frac{3x^2y^3 - 3x^3y^2(-\frac{x^3}{y^3})}{y^6}$
    - $= -\frac{3(x^2y^4 + x^6)}{y^7} = -\frac{3x^2(y^4 + x^4)}{y^7}$
  - Answer simplifies to
    - $y'' = -\frac{3x^2(16)}{y^7} = -48\frac{x^2}{y^7}$